

Quantum Mechanics I - PSet 6

Telmo Cunha

November 2025

Exercise 1

Consider the following wavefunction for a particle of mass m in an infinite square well of width a

$$\Psi(x, 0) = \frac{1}{\sqrt{3}} \sqrt{\frac{2}{a}} \sin\left(\frac{2\pi x}{a}\right) + \frac{2}{\sqrt{3}} \sqrt{\frac{2}{a}} \sin\left(\frac{3\pi x}{a}\right). \quad (1.1)$$

- (a) For $\Psi(x, 0)$ to be an energy eigenstate it needs to satisfy the eigenvalue equation for the Hamiltonian operator, i.e.

$$\hat{H}\Psi(x, 0) = E\Psi(x, 0), \quad (1.2)$$

or equivalently

$$\hat{H}\Psi(x, 0) - E\Psi(x, 0) = 0. \quad (1.3)$$

Instead of verifying this let us compute directly the eigenstates for the infinite square-well of width a . Let $\psi(x) := \Psi(x, 0)$, the TISE is given by

$$-\frac{\hbar^2}{2m} \frac{d^2\psi(x)}{dx^2} = E\psi(x), \quad (1.4)$$

with solutions

$$\psi(x) = A \sin(kx) + B \cos(kx), \quad (1.5)$$

where $k = \sqrt{2mE}/\hbar$. From the boundary data $\psi(0) = \psi(a) = 0$, we have $B = 0$ and

$$ka = n\pi, \quad (1.6)$$

where we consider $n \in \mathbb{N}$ since $\sin(-\alpha) = -\sin(\alpha)$, giving the same state. This leads to

$$E_n = \frac{n^2 \pi^2 \hbar^2}{2ma^2}, \quad n \in \mathbb{N}. \quad (1.7)$$

We find A by enforcing normalization, i.e.

$$1 = |A|^2 \int_0^a \sin^2(kx) dx = |A|^2 \frac{a}{2}, \quad (1.8)$$

which, considering $A \in \mathbb{R}$, leads to $A = \sqrt{2/a}$. To conclude, the energy eigenstates are given by

$$\psi_n(x) = \sqrt{\frac{2}{a}} \sin\left(\frac{n\pi x}{a}\right), \quad n \in \mathbb{N}. \quad (1.9)$$

Clearly, $\Psi(x, 0)$ is a linear combination of the eigenstates $\psi_2(x)$ and $\psi_3(x)$ and therefore it is not an energy eigenstate. To find $\Psi(x, t)$ we just need to add the time dependence corresponding to each

eigenstate, since each one separately is a solution and Schrödinger's equation is linear, i.e. linear combinations are also solutions. We have then

$$\Psi(x, t) = \frac{1}{\sqrt{3}} \sqrt{\frac{2}{a}} \sin\left(\frac{2\pi x}{a}\right) e^{-\frac{iE_2 t}{\hbar}} + \frac{2}{\sqrt{3}} \sqrt{\frac{2}{a}} \sin\left(\frac{3\pi x}{a}\right) e^{-\frac{iE_3 t}{\hbar}}. \quad (1.10)$$

Briefly, recall that we consider solutions of the form $\Psi(x, t) = f(x)g(t)$ leading to two equations, one for t and one for x , each equal to the same constant E .

- (b) By the measurement postulate the probability of measuring the energy corresponding to state n is $|c_n|^2$, where c_n is the coefficient of eigenstate n . For $n = 1$ since its coefficient in $\Psi(x, 0)$ is zero, the probability is zero. For $n = 2$ this corresponds to $1/3$ and for $n = 3$ it is $2/3$, summing to 1 as it should.
- (c) We have

$$\Psi(x, t) = c_2 \psi_2(x) e^{-\frac{iE_2 t}{\hbar}} + c_3 \psi_3(x) e^{-\frac{iE_3 t}{\hbar}}, \quad (1.11)$$

$c_2, c_3 \in \mathbb{R}$. Thus

$$\begin{aligned} \langle \hat{x} \rangle(t) &= \langle \Psi(x, t) | x | \Psi(x, t) \rangle \\ &= \int_0^a \left[c_2^2 x \psi_2^2 + c_3^2 x \psi_3^2 + c_2 c_3 \psi_2 \psi_3 x e^{-i(E_3 - E_2)t/\hbar} \right. \\ &\quad \left. + c_2 c_3 \psi_2 \psi_3 x e^{-i(E_2 - E_3)t/\hbar} \right] dx \\ &= \int_0^a \left[c_2^2 x \psi_2^2 + c_3^2 x \psi_3^2 + 2\Re \left(c_2 c_3 e^{-i(E_3 - E_2)t/\hbar} \langle \psi_2 | x | \psi_3 \rangle \right) \right] dx. \end{aligned} \quad (1.12)$$

The first two terms are of the form

$$\begin{aligned} c_n^2 \int_0^a x \psi_n^2 dx &= c_n^2 \int_0^a x \frac{2}{a} \sin^2\left(\frac{n\pi x}{a}\right) dx = \frac{2c_n^2}{a} \int_0^a x \left(\frac{1 - \cos(2n\pi x/a)}{2} \right) dx \\ &= \frac{2c_n^2}{a} \left[\frac{a^2}{4} - \int_0^a x \left(\frac{\cos(2n\pi x/a)}{2} \right) dx \right] \\ &= \frac{2c_n^2}{a} \left[\frac{a^2}{4} - \frac{1}{2} \int_0^a x \cos(2n\pi x/a) dx \right] \\ &= \frac{2c_n^2}{a} \left[\frac{a^2}{4} - \frac{1}{2} \left(\frac{a}{2n\pi} x \sin(2n\pi x/a) \right) \Big|_0^a - \frac{a}{2n\pi} \int_0^a \sin(2n\pi x/a) dx \right] \\ &= \frac{2c_n^2}{a} \left[\frac{a^2}{4} - \frac{1}{2} \left(\frac{a}{2n\pi} x \sin(2n\pi x/a) \right) \Big|_0^a + \frac{a^2}{4n^2\pi^2} \cos(2n\pi x/a) \Big|_0^a \right] \\ &= c_n^2 \frac{a}{2}, \end{aligned} \quad (1.13)$$

while

$$\begin{aligned} \langle \psi_n | x | \psi_m \rangle &= \frac{2}{a} \int_0^a x \sin\left(\frac{n\pi x}{a}\right) \sin\left(\frac{m\pi x}{a}\right) dx \\ &= \frac{1}{a} \int_0^a x \cos\left(\frac{n\pi x}{a} - \frac{m\pi x}{a}\right) - x \cos\left(\frac{n\pi x}{a} + \frac{m\pi x}{a}\right) dx \\ &= \frac{1}{a} \int_0^a x \cos\left(\frac{(n-m)\pi x}{a}\right) - x \cos\left(\frac{(n+m)\pi x}{a}\right) dx, \end{aligned} \quad (1.14)$$

which leads to

$$\begin{aligned}
\int_0^a x \cos(k\pi x/a) dx &= \frac{a}{k\pi} x \sin(k\pi x/a) \Big|_0^a - \frac{a}{k\pi} \int_0^a \sin(k\pi x/a) dx \\
&= \frac{a^2}{k^2\pi^2} \cos(k\pi x/a) \Big|_0^a dx \\
&= \begin{cases} -\frac{2a^2}{k^2\pi^2}, & \text{if } k \text{ is odd,} \\ 0, & \text{if } k \text{ is even.} \end{cases}
\end{aligned} \tag{1.15}$$

So, the integral above becomes

$$\langle \psi_n | x | \psi_m \rangle = \begin{cases} \frac{2a}{\pi^2} \left(\frac{1}{(n+m)^2} - \frac{1}{(n-m)^2} \right), & \text{if } n-m \text{ (and thus } n+m) \text{ is odd,} \\ 0, & \text{if } n-m \text{ (and thus } n+m) \text{ is even,} \end{cases} \tag{1.16}$$

In particular

$$\langle \psi_2 | x | \psi_3 \rangle = -\frac{48a}{25\pi^2}. \tag{1.17}$$

Finally, we have

$$\langle \hat{x} \rangle(t) = \frac{a}{2} - \frac{32\sqrt{2}a}{25\pi^2} \cos\left(\frac{5\pi^2\hbar}{2ma^2}t\right). \tag{1.18}$$

- (d) Similarly, we have

$$\begin{aligned}
\langle \hat{p} \rangle(t) &= -i\hbar \int_0^a \left[c_2^2 \psi_2 \psi_2' + c_3^2 \psi_3 \psi_3' + c_2 c_3 \psi_2 \psi_3' e^{-i(E_2-E_3)\frac{t}{\hbar}} + c_2 c_3 \psi_2' \psi_3 e^{-i(E_3-E_2)\frac{t}{\hbar}} \right] dx \\
&= -i\hbar c_2 c_3 e^{-i(E_2-E_3)\frac{t}{\hbar}} \int_0^a (\psi_2 \psi_3') dx - i\hbar c_2 c_3 e^{-i(E_3-E_2)\frac{t}{\hbar}} \int_0^a (\psi_2' \psi_3) dx \\
&= i\hbar A c_2 c_3 (e^{i\omega t} - e^{-i\omega t}) \\
&= 2\hbar c_2 c_3 A \sin(\omega t) \\
&= \frac{16\sqrt{2}\hbar}{5a} \sin\left(\frac{E_3 - E_2}{\hbar}t\right) \\
&= \frac{16\sqrt{2}\hbar}{5a} \sin\left(\frac{5\pi^2\hbar}{2ma^2}t\right),
\end{aligned} \tag{1.19}$$

where we use $\sin(a)\cos(b) = 1/2(\sin(a+b) + \sin(a-b))$ and define A as

$$\begin{aligned}
A &:= \int_0^a \psi_2 \psi_3' dx = \frac{6\pi}{a^2} \int_0^a \sin\left(\frac{2\pi x}{a}\right) \cos\left(\frac{3\pi x}{a}\right) dx \\
&= \frac{3\pi}{a^2} \int_0^a \sin\left(\frac{5\pi x}{a}\right) - \sin\left(\frac{\pi x}{a}\right) dx \\
&= \frac{3\pi}{a^2} \left(\frac{2a}{5\pi} - \frac{2a}{\pi} \right) \\
&= -\frac{24}{5a},
\end{aligned} \tag{1.20}$$

using the fact that

$$\int_0^a \psi_n \psi_n' dx = \sqrt{\frac{a}{2}} \psi_n^2(x) \Big|_0^a = 0, \tag{1.21}$$

and also that

$$\int_0^a \psi_n \psi'_m dx = - \int_0^a \psi'_n \psi_m dx, \quad (1.22)$$

using integration by parts and the fact that the wavefunctions vanish at the boundary. Thus, we conclude that

$$\langle \hat{p} \rangle(t) = \frac{16\sqrt{2}\hbar}{5a} \sin\left(\frac{5\pi^2\hbar}{2ma^2}t\right). \quad (1.23)$$

Exercise 2

This corresponds to exercise 2.44, page 78, of [GS18]. Prove the following: In one dimension ($-\infty < x < \infty$) there are no degenerate bound states (where scalar multiples of a solution is considered to be the same solution).

Suppose we have bound states ψ_1 and ψ_2 with the same energy E and such that $\psi_1 \neq \psi_2$. Then

$$\begin{cases} \hat{H}\psi_1 = E\psi_1, \\ \hat{H}\psi_2 = E\psi_2, \end{cases} \quad (1.24)$$

equivalently

$$\begin{cases} \frac{d^2\psi_1}{dx^2} = -\frac{2mE}{\hbar^2}\psi_1 + \frac{2m}{\hbar^2}V(x)\psi_1, \\ \frac{d^2\psi_2}{dx^2} = -\frac{2mE}{\hbar^2}\psi_2 + \frac{2m}{\hbar^2}V(x)\psi_2. \end{cases} \quad (1.25)$$

Multiply the first equation by ψ_2 , the second by ψ_1 and subtract to obtain

$$\psi_1''\psi_2 - \psi_2''\psi_1 = \frac{d}{dx}(\psi_1'\psi_2 - \psi_2'\psi_1) = 0. \quad (1.26)$$

Therefore

$$\psi_1'\psi_2 - \psi_2'\psi_1 = C, \quad (1.27)$$

for some $C \in \mathbb{R}$. Since we are considering bound states, which are normalizable, they decay to zero at infinity, therefore we must in fact have $C = 0$. In a neighborhood of x_0 such that $\psi_1(x) \neq 0$, by continuity and because otherwise $\psi_1(x) \equiv 0$, we have

$$\left(\frac{\psi_2}{\psi_1}\right)' = \frac{\psi_2\psi_1'}{\psi_1^2} - \frac{\psi_2'\psi_1}{\psi_1^2} = \frac{C}{\psi_1^2} = 0. \quad (1.28)$$

Integrating from x_0 to x we obtain

$$\psi_2(x) = \frac{\psi_2(x_0)}{\psi_1(x_0)}\psi_1(x) =: c\psi_1(x), \quad (1.29)$$

around a neighborhood of x_0 . Consider now

$$f(x) := \psi_2(x) - c\psi_1(x), \quad (1.30)$$

where $f(x_0) = 0$ by definition, and

$$f'(x_0) = \frac{\psi_1(x_0)}{\psi_1(x_0)}\psi_2'(x_0) - \frac{\psi_2(x_0)}{\psi_1(x_0)}\psi_1'(x_0) = 0. \quad (1.31)$$

Because ψ_1 and ψ_2 solve the same linear second order ODE so does f , since it is a linear combination. Therefore, the IVP with initial data $f(x_0) = 0$ and $f'(x_0) = 0$ implies $f(x) \equiv 0$ is the unique solution for all x and thus

$$\psi_2(x) = c\psi_1(x), \quad \forall x \in \mathbb{R}, \quad (1.32)$$

concluding the proof.

Exercise 3

- (a) The 2D TISE within the well is given by

$$-\frac{\hbar^2}{2m}\Delta\psi(x, y) = E\psi(x, y), \quad (1.33)$$

which we solve using the usual separation of variables trick. Suppose

$$\psi(x, y) = f(x)g(y), \quad (1.34)$$

then

$$\frac{f''(x)}{f(x)} + \frac{g''(y)}{g(y)} = -\frac{2mE}{\hbar^2}. \quad (1.35)$$

This implies that

$$\begin{cases} f''(x) = Af(x), \\ g''(y) = Bg(y), \end{cases} \quad (1.36)$$

for some constants $A, B \in \mathbb{R}$ and such that

$$A + B = -\frac{2mE}{\hbar^2}. \quad (1.37)$$

Depending on the sign of A and B one can have several different solutions. However, for the solution to represent a bound state, we can not have exponential terms since those do not satisfy the boundary condition. From the boundary conditions we have that

$$f(0) = f(L_x) = 0. \quad (1.38)$$

Suppose $A > 0$, then

$$f(x) = e^{Ax} + e^{-Ax}. \quad (1.39)$$

However, in this case, $f(0) \neq 0$. Similarly, if $A = 0$, we have

$$f(x) = Cx + D, \quad (1.40)$$

and from $f(0) = 0$ we have $D = 0$ and from $f(L_x) = 0$ we have $C = 0$, which gives the trivial solution. Thus, we must have $A < 0$ and we define $A = -k_x^2$ leading to

$$f(x) = A_x \sin(k_x x) + B_x \cos(k_x x). \quad (1.41)$$

From $f(0) = 0$ we have $B_x = 0$ and from $f(L_x) = 0$ we have

$$k_x = \frac{n_x \pi}{L_x}, \quad (1.42)$$

$n_x \in \mathbb{N}$. Similarly, defining $B = -k_y^2$, for $g(y)$ we have

$$g(y) = A_y \sin(k_y y), \quad (1.43)$$

and from $g(L_y) = 0$ we have

$$k_y = \frac{n_y \pi}{L_y}, \quad (1.44)$$

$n_y \in \mathbb{N}$. Then, we have

$$\frac{2mE}{\hbar^2} = \frac{n_x^2 \pi^2}{L_x^2} + \frac{n_y^2 \pi^2}{L_y^2}, \quad (1.45)$$

for $n_x, n_y \in \mathbb{N}$ leading to

$$E = \frac{\pi^2 \hbar^2}{2m} \left(\frac{n_x^2}{L_x^2} + \frac{n_y^2}{L_y^2} \right), \quad n_x = 1, 2, 3, \dots, \quad n_y = 1, 2, 3, \dots \quad (1.46)$$

The eigenfunctions are given by

$$\psi(x, y) = A_x A_y \sin\left(\frac{n_x \pi}{L_x} x\right) \sin\left(\frac{n_y \pi}{L_y} y\right). \quad (1.47)$$

The normalization conditions gives

$$\begin{aligned} 1 &= A_x^2 A_y^2 \int_0^{L_x} \sin^2\left(\frac{n_x \pi}{L_x} x\right) dx \int_0^{L_y} \sin^2\left(\frac{n_y \pi}{L_y} y\right) dy \\ &= A_x^2 A_y^2 \frac{L_x}{2} \frac{L_y}{2}, \end{aligned} \quad (1.48)$$

Thus

$$A_x A_y = \frac{2}{\sqrt{L_x L_y}}, \quad (1.49)$$

and the normalized eigenstates are

$$\psi_{n_x, n_y}(x, y) = \frac{2}{\sqrt{L_x L_y}} \sin\left(\frac{n_x \pi}{L_x} x\right) \sin\left(\frac{n_y \pi}{L_y} y\right), \quad n_x, n_y \in \mathbb{N}, \quad (1.50)$$

with energies

$$E(n_x, n_y) = \frac{\pi^2 \hbar^2}{2m} \left(\frac{n_x^2}{L_x^2} + \frac{n_y^2}{L_y^2} \right), \quad n_x, n_y \in \mathbb{N}. \quad (1.51)$$

- (b) Suppose that $L_x = L_y = L$, then the eigenfunctions are given by

$$\psi_{n_x, n_y}(x, y) = \frac{2}{L} \sin\left(\frac{n_x \pi}{L} x\right) \sin\left(\frac{n_y \pi}{L} y\right), \quad n_x, n_y \in \mathbb{N}, \quad (1.52)$$

with energies

$$E(n_x, n_y) = \frac{\pi^2 \hbar^2}{2m} \left(\frac{n_x^2 + n_y^2}{L^2} \right), \quad n_x, n_y \in \mathbb{N}. \quad (1.53)$$

The simple symmetry consideration comes from switching n_x with n_y , i.e. $E(n_x, n_y) = E(n_y, n_x)$. However, there are other “accidental” symmetries, the given example is $n_x = 7, n_y = 1$ and $n_x = 5, n_y = 5$, leading to the same energy. Another such example is $n_x = 10, n_y = 5$ and $n_x = 2, n_y = 11$ since $10^2 + 5^2 = 11^2 + 2^2 = 125$.

- (c) We have

$$E(n_x, n_y) = \frac{\pi^2 \hbar^2}{2m} \left(\frac{L_y^2 n_x^2 + L_x^2 n_y^2}{L_y^2 L_x^2} \right), \quad n_x, n_y \in \mathbb{N}. \quad (1.54)$$

To have a degeneracy we must have

$$L_y^2 n_x^2 + L_x^2 n_y^2 = L_y^2 a + L_x^2 b = L_y^2 c + L_x^2 d, \quad (1.55)$$

for some $a, b, c, d \in \mathbb{N}$ with $(a, b) \neq (c, d)$. However, this leads to

$$\frac{L_x^2}{L_y^2} = \frac{c - a}{b - d}, \quad (1.56)$$

which is impossible since the LHS is an irrational number and the RHS is a rational number. When $b = d$ we have immediately $a = c$ so there is never degeneracy in this case.

Exercise 4

We are given the potential

$$V(x) = \begin{cases} \infty, & \text{for } x < 0 \\ 0, & \text{for } 0 < x < a \\ V_0, & \text{for } a < x < 2a \\ \infty, & \text{for } x > 2a \end{cases} \quad (1.57)$$

- (a) The TISE for $0 < x < a$ is given by

$$\psi_1''(x) = -\frac{2mE}{\hbar^2} \psi_1(x), \quad (1.58)$$

with solutions

$$\psi_1(x) = A \sin(kx) + B \cos(kx). \quad (1.59)$$

The boundary data $\psi_1(0) = 0$ forces $B = 0$ and thus

$$\psi_1(x) = A \sin(kx), \quad 0 \leq x < a. \quad (1.60)$$

The TISE for $a < x < 2a$ is given by

$$\psi_2''(x) = \frac{2m(V_0 - E)}{\hbar^2} \psi_2(x), \quad (1.61)$$

where $0 < E < V_0$. Thus, the solutions are of the form

$$\psi_2(x) = C e^{\kappa x} + D e^{-\kappa x}. \quad (1.62)$$

The boundary data $\psi_2(2a) = 0$ gives

$$C e^{2\kappa a} + D e^{-2\kappa a} = 0, \quad (1.63)$$

leading to

$$-\frac{D}{C} = e^{4\kappa a}, \quad (1.64)$$

or

$$D = -C e^{4\kappa a}, \quad (1.65)$$

and thus

$$\psi_2(x) = C \left(e^{\kappa x} - e^{\kappa(4a-x)} \right). \quad (1.66)$$

We further have

$$\psi_1(a) = \psi_2(a) \quad (1.67)$$

leading to

$$A \sin(ka) = C \left(e^{\kappa a} - e^{3\kappa a} \right). \quad (1.68)$$

and

$$\psi_1'(a) = \psi_2'(a) \quad (1.69)$$

leading to

$$kA \cos(ka) = \kappa C \left(e^{\kappa a} + e^{3\kappa a} \right). \quad (1.70)$$

Dividing (1.68) by (1.70) we obtain

$$\tan(ka) = \frac{k}{\kappa} \frac{e^{\kappa a} - e^{3\kappa a}}{e^{\kappa a} + e^{3\kappa a}}. \quad (1.71)$$

From

$$\begin{cases} \eta = ka, \\ \xi = \kappa a, \end{cases} \quad (1.72)$$

and

$$\xi^2 + \eta^2 = z_0^2, \quad (1.73)$$

we have

$$\frac{\tan(\eta)}{\eta} = \frac{1}{\xi} \frac{e^{\xi} - e^{3\xi}}{e^{\xi} + e^{3\xi}} = \left(\frac{1}{\xi} \right) \frac{1 - e^{2\xi}}{1 + e^{2\xi}} = -\frac{\tanh(\xi)}{\xi}. \quad (1.74)$$

So, we have the two equations

$$\begin{cases} \frac{\tan(\eta)}{\eta} = -\frac{\tanh(\xi)}{\xi}, \\ \xi^2 + \eta^2 = z_0^2 = \frac{2ma^2 V_0}{\hbar^2}. \end{cases} \quad (1.75)$$

- (b) We have

$$\xi = \sqrt{z_0^2 - \eta^2}, \quad (1.76)$$

since $\xi > 0$. Solving these equations for $z_0 = 2\pi$ leads to a unique solution

$$\eta \approx 5.28. \quad (1.77)$$

Thus, we have a single state. Since we do not know a we can only specify E in terms of V_0 where

$$\frac{E}{V_0} = \frac{\hbar^2 \eta^2 / (2ma^2)}{\hbar^2 z_0^2 / (2ma^2)} = \frac{\eta^2}{z_0^2} \approx 0.7075. \quad (1.78)$$

Exercise 5

Computational (to solve later).

Exercise 6

Computational (to solve later).

References

- [GS18] David J. Griffiths and Darrell F. Schroeter. *Introduction to quantum mechanics*. Third edition. Cambridge ; New York, NY: Cambridge University Press, 2018. ISBN: 978-1-107-18963-8.